Prepare for a operation SysF semantic

Types/Utils.lean
@@ -2,3 +2,5 @@ open Lean in
 instance : HAdd NumLit Nat NumLit where
   hAdd x n := Syntax.mkNumLit s!"{x.getNat + n}"
 
+def Nat.split : ∀ n, ∃ a b : Nat, n = a + b := fun n => ⟨n, 0, rfl⟩
+
