Types/Expr/TRefSet.lean
@@ -1,0 +1,69 @@
+import Types.Expr.Stx
+import Types.Ty.RefSet
+
+namespace Expr
+
+-- TRefSet predicate for expressions - tracks type variable references
+@[grind]
+inductive TRefSet : Expr → Nat → Prop
+  | appL {a b idx} : TRefSet a idx → TRefSet (.app a b) idx
+  | appR {a b idx} : TRefSet b idx → TRefSet (.app a b) idx
+  | lamT {ty body idx} : Ty.RefSet ty idx → TRefSet (.lam ty body) idx
+  | lamB {ty body idx} : TRefSet body idx → TRefSet (.lam ty body) idx
+  | tappL {expr ty idx} : TRefSet expr idx → TRefSet (.tapp expr ty) idx
+  | tappR {expr ty idx} : Ty.RefSet ty idx → TRefSet (.tapp expr ty) idx
+  | tlam {body idx} : TRefSet body idx.succ → TRefSet (.tlam body) idx
+
+@[simp, grind =]
+theorem TRefSet_lam {ty body idx} : TRefSet (.lam ty body) idx ↔ (Ty.RefSet ty idx ∨ TRefSet body idx) := by
+  grind
+
+@[simp, grind =]
+theorem TRefSet_tlam {body idx} : TRefSet (.tlam body) idx ↔ TRefSet body (idx + 1) := by
+  grind
+
+@[simp, grind =]
+theorem TRefSet_app {a b idx} : TRefSet (.app a b) idx ↔ (TRefSet a idx ∨ TRefSet b idx) := by
+  grind
+
+@[simp, grind =]
+theorem TRefSet_tapp {expr ty idx} : TRefSet (.tapp expr ty) idx ↔ (TRefSet expr idx ∨ Ty.RefSet ty idx) := by
+  grind
+
+@[simp]
+theorem TRefSet_id {idx jdx} : ¬TRefSet (.id idx) jdx := by
+  grind
+
+example : TRefSet (.lam [t|0] (.id 1)) 0 := .lamT .id
+example : TRefSet (.tapp (.id 0) [t|1]) 1 := .tappR .id
+example : TRefSet (.tlam (.tapp (.id 0) [t|1])) 0 := .tlam (.tappR .id)
+example : ¬∃ n, TRefSet (.id 5) n := by simp
+
+theorem TRefSet_dist_app {ty a b idx} : TRefSet (.lam ty (.app a b)) idx ↔ TRefSet (.lam ty a) idx ∨ TRefSet (.lam ty b) idx := by
+  grind
+
+theorem TRefSet_dist_tlam {a b idx} : TRefSet (.tlam (.app a b)) idx ↔ TRefSet (.tlam a) idx ∨ TRefSet (.tlam b) idx := by
+  grind
+
+instance TRefSet.dec : {e : Expr} → {n : Nat} → Decidable (TRefSet e n)
+  | .id x, v => .isFalse $ by simp
+  | .lam ty b, v =>
+    match Ty.RefSet.dec (t := ty) (n := v), @TRefSet.dec b v with
+    | .isTrue h, _ => .isTrue <| .lamT h
+    | _, .isTrue h => .isTrue <| .lamB h
+    | .isFalse h₁, .isFalse h₂ => .isFalse $ by simp_all
+  | .tlam b, v => match @TRefSet.dec b v.succ with
+    | .isTrue h => .isTrue <| .tlam h
+    | .isFalse h => .isFalse <| by simpa
+  | .app a b, v =>
+    match @TRefSet.dec a v, @TRefSet.dec b v with
+    | .isTrue h, _ => .isTrue <| .appL h
+    | _, .isTrue h => .isTrue <| .appR h
+    | .isFalse h₁, .isFalse h₂ => .isFalse $ by simp_all
+  | .tapp expr ty, v =>
+    match @TRefSet.dec expr v, Ty.RefSet.dec (t := ty) (n := v) with
+    | .isTrue h, _ => .isTrue <| .tappL h
+    | _, .isTrue h => .isTrue <| .tappR h
+    | .isFalse h₁, .isFalse h₂ => .isFalse $ by simp_all
+
+end Expr
