Types/Ty/E.lean
@@ -1,0 +1,35 @@
+import Types.Ty.Valid
+
+namespace Ty
+
+/-- An extrinsically valid Ty -/
+structure E (n : Nat) where
+  mk ::
+  ty : Ty
+  val : Valid n ty
+
+namespace E
+
+variable {n : Nat}
+
+@[match_pattern] abbrev fn : E n → E n → E n := (.mk _ $ .fn ·.val ·.val)
+@[match_pattern] abbrev fa : E (n + 1) → E n := (.mk _ $ .fa ·.val)
+@[match_pattern] abbrev id : Fin n     → E n := (.mk _ $ .id ·)
+
+@[simp]
+def fn.injEq {a b c d : E n} : E.fn a b = E.fn c d ↔ (a = c ∧ b = d) := by
+  cases a; cases b; cases c; cases d; grind
+
+@[simp]
+def fa.injEq {a b : E n.succ} : E.fa a = E.fa b ↔ (a = b) := by
+  cases a; cases b; grind
+
+@[simp]
+def id.injEq {a b : Fin n} : E.id a = E.id b ↔ (a = b) := by grind
+
+def bvarShift (shift skip : Nat) (x : E n) : E (n + shift) :=
+  .mk _ $ Valid.bvarShift (skip := skip) x.val
+
+def replace (hbody : E n.succ) (hrepl : E n) : E n :=
+  .mk _ $ Valid.replace hbody.val hrepl.val
+
