Types/Ty/RefSet.lean
@@ -3,6 +3,7 @@ import Types.Ty.Stx
 namespace Ty
 
 -- RefSet predicate for types
+@[grind]
 inductive RefSet : Ty → Nat → Prop
   | fnL {a b idx} : RefSet a idx → RefSet (.fn a b) idx
   | fnR {a b idx} : RefSet b idx → RefSet (.fn a b) idx
@@ -11,30 +12,28 @@ inductive RefSet : Ty → Nat → Prop
 
 @[simp]
 theorem RefSet_fa {body idx} : RefSet (.fa body) idx ↔ RefSet body (idx + 1) := by
-  constructor
-  <;> intro h
-  · cases h; assumption
-  · exact .fa h
+  grind
 
 @[simp]
 theorem RefSet_fn {a b idx} : RefSet (.fn a b) idx ↔ (RefSet a idx ∨ RefSet b idx) := by
-  constructor
-  <;> rintro (h|h)
-  · exact .inl h
-  · exact .inr h
-  · exact .fnL h
-  · exact .fnR h
+  grind
 
 @[simp]
 theorem RefSet_id {idx jdx} : RefSet (.id idx) jdx ↔ idx = jdx := by
-  constructor
-  <;> intro h
-  · cases h; rfl
-  · rw [h]
-    exact .id
+  grind
 
 theorem RefSet_dist {a b idx} : RefSet (.fa (.fn a b)) idx ↔ RefSet (.fa a) idx ∨ RefSet (.fa b) idx := by
-  constructor
-  <;> intro h
-  <;> simp only [RefSet_fa, RefSet_fn] at h ⊢
-  <;> exact h
+  grind
+
+instance RefSet.dec : {t : Ty} → {n : Nat} → Decidable (RefSet t n)
+  | .id x, v => if h : x = v then .isTrue <| h ▸ .id
+    else .isFalse $ by simpa
+  | .fa b, v => match @RefSet.dec b v.succ with
+    | .isTrue h => .isTrue <| .fa h
+    | .isFalse h => .isFalse <| by simpa
+  | .fn a b, v =>
+    match @RefSet.dec a v, @RefSet.dec b v with
+    | .isTrue h, _ => .isTrue <| .fnL h
+    | _, .isTrue h => .isTrue <| .fnR h
+    | .isFalse h₁, .isFalse h₂ => .isFalse $ by simp_all
+
